progress

HOL_To_IMP/Refinements/HOL_TCN_To_IMP_Temp.thy
@@ -59,6 +59,182 @@ lemma compiler_correct_nt:
   sorry
 
 
+
+
+(* TODO: this should (just?) use the small step semantics instead !!!! *)
+(* state, term, constants, calls, new state, tail call *)
+inductive tto_end :: "state \<Rightarrow> tcom \<Rightarrow> nat \<Rightarrow> (com \<times> state) list \<Rightarrow> state \<Rightarrow> bool \<Rightarrow> bool" where
+  "tto_end s tSKIP (Suc 0) [] s False" |
+  "tto_end s (tAssign x a) (Suc (Suc 0)) [] (s(x := aval a s)) False" |
+  "\<lbrakk>tto_end s1 c1 k1 gs1 s2 False; tto_end s2 c2 k2 gs2 s3 l2; k = k1 + k2; gs = gs1 @ gs2\<rbrakk>
+    \<Longrightarrow> tto_end s1 (tSeq c1 c2) k gs s3 l2" | (* l1 = False ? *)
+  "\<lbrakk>s b \<noteq> 0; tto_end s c1 x gs t l; y = x + 1\<rbrakk> \<Longrightarrow> tto_end s (tIf b c1 c2) y gs t l" |
+  "\<lbrakk>s b = 0; tto_end s c2 x gs t l; y = x + 1\<rbrakk> \<Longrightarrow> tto_end s (tIf b c1 c2) y gs t l" |
+  "\<lbrakk>(C,s) \<Rightarrow>\<^bsup>z \<^esup> t\<rbrakk> \<Longrightarrow> tto_end s (tCall C r) 0 [(C,s)] (s(r := t r)) False" |
+  "tto_end s tTAIL 5 [] s True"
+
+
+(*
+lemma tto_end_tseqs:
+  assumes "\<forall>i \<le> length cs. tto_end s (cs ! i) (ks ! i) (gss ! i)"
+  shows True *)
+
+fun tcalls where
+  "tcalls (tSeq c1 c2) = tcalls c1 @ tcalls c2" |
+  "tcalls (tIf x c1 c2) = tcalls c1 @ tcalls c2" |
+  "tcalls (tCall C r) = [C]" |
+  "tcalls _ = []"
+
+definition "truntime_reg gs T_g = (\<forall>C \<in> gs. \<forall>s. \<exists>t. (C,s) \<Rightarrow>\<^bsup> T_g C s \<^esup> t)"
+definition "tinterp_time2 T_g k gs = k + sum_map (\<lambda>(C,s). T_g C s) gs"
+
+lemma tinterp_time2_nil: "tinterp_time2 T_g k [] = k" unfolding tinterp_time2_def by simp
+
+theorem tto_end_non_tail:
+  fixes p :: tcom
+  assumes "truntime_reg (set (tcalls p)) T_g"
+  assumes "tto_end s p k gs t l"
+  assumes "l = False"
+  shows "tp \<turnstile> (p,s) \<Rightarrow>\<^bsup>tinterp_time2 T_g k gs\<^esup> t"
+using assms(2,1,3) proof (induction rule: tto_end.induct)
+  case (1 s)
+  then show ?case using tinterp_time2_nil tSkip by metis
+next
+  case (2 s x a) show ?case using tinterp_time2_nil tAssign by metis
+next
+  case (3 s1 c1 k1 gs1 s2 c2 k2 gs2 s3 l2 k gs)
+
+  have *: "tinterp_time2 T_g k gs = tinterp_time2 T_g k1 gs1 + tinterp_time2 T_g k2 gs2"
+    unfolding tinterp_time2_def using \<open>k = k1 + k2\<close> \<open>gs = gs1 @ gs2\<close> by simp
+
+  have **: "truntime_reg (set (tcalls c1)) T_g" "truntime_reg (set (tcalls c2)) T_g"
+    using "3.prems" unfolding truntime_reg_def by auto
+  
+  from 3 * ** show ?case by blast
+next
+  case (4 s b c1 x gs t l y c2)
+  then have "truntime_reg (set (tcalls c1)) T_g" unfolding truntime_reg_def by auto
+  with 4 show ?case unfolding tinterp_time2_def by auto
+next
+  case (5 s b c2 x gs t l y c1)
+  then have "truntime_reg (set (tcalls c2)) T_g" unfolding truntime_reg_def by auto
+  with 5 show ?case unfolding tinterp_time2_def by auto
+next
+  case (6 C s z t r)
+  show ?case
+    apply (rule tCall) unfolding tinterp_time2_def apply simp
+    using 6 unfolding truntime_reg_def using bigstep_det by force (* TODO: cleanup *)
+next
+  case (7 s)
+  then show ?case by blast
+qed
+
+theorem tto_end_tail:
+  fixes p1 p2 :: tcom
+  assumes "truntime_reg (set (tcalls p1)) T_g"
+  assumes "p2 \<turnstile> (p1,s1) \<Rightarrow>\<^bsup>z\<^esup> t"
+  assumes "tto_end s1 p1 k gs s2 l"
+  assumes "l = True"
+  shows "\<exists>z2. z = tinterp_time2 T_g k gs + z2 \<and> p2 \<turnstile> (p2,s2) \<Rightarrow>\<^bsup>z2\<^esup> t"
+using assms(3,1,2,4) proof (induction arbitrary: z rule: tto_end.induct)
+  case (1 s) then show ?case by blast
+next
+  case (2 s x a) then show ?case by blast
+next
+  case (3 s1 c1 k1 gs1 s2 c2 k2 gs2 s3 l2 k gs)
+
+  have *: "tinterp_time2 T_g k gs = tinterp_time2 T_g k1 gs1 + tinterp_time2 T_g k2 gs2"
+    unfolding tinterp_time2_def using \<open>k = k1 + k2\<close> \<open>gs = gs1 @ gs2\<close> by simp
+  have **: "truntime_reg (set (tcalls c1)) T_g" "truntime_reg (set (tcalls c2)) T_g"
+    using "3.prems" unfolding truntime_reg_def by auto
+
+  have "p2 \<turnstile> (c1,s1) \<Rightarrow>\<^bsup>tinterp_time2 T_g k1 gs1\<^esup>  s2" using tto_end_non_tail ** 3 by blast
+  then obtain y where tSeq_inv:
+    "z = tinterp_time2 T_g k1 gs1 + y"
+    "p2 \<turnstile> (c1, s1) \<Rightarrow>\<^bsup>tinterp_time2 T_g k1 gs1\<^esup> s2"
+    "p2 \<turnstile> (c2, s2) \<Rightarrow>\<^bsup>y\<^esup> t"
+    using tSeq_tE "3.prems" tdeterm by metis
+  then obtain z2 where "y = tinterp_time2 T_g k2 gs2 + z2" "p2 \<turnstile> (p2, s3) \<Rightarrow>\<^bsup>z2\<^esup> t"
+    using "3.IH" \<open>l2 = True\<close> ** by blast
+  then show ?case using tSeq_inv * by simp
+next
+  case (4 s b c1 x gs t l y c2)
+  then have "truntime_reg (set (tcalls c1)) T_g" unfolding truntime_reg_def apply simp by blast
+  with 4 show ?case unfolding tinterp_time2_def by auto
+next
+  case (5 s b c2 x gs t l y c1)
+  then have "truntime_reg (set (tcalls c2)) T_g" unfolding truntime_reg_def apply simp by blast
+  with 5 show ?case unfolding tinterp_time2_def by auto
+next
+  case (6 C s z t r)
+  then show ?case by blast
+next
+  case (7 s)
+  then show ?case using tinterp_time2_nil by force
+qed
+
+lemma tto_end_struct_k:
+  assumes "tto_end s c k gs t l"
+  shows "k \<le> tstruct_k c"
+  using assms by (induction rule: tto_end.induct) simp_all
+
+thm tto_end_non_tail tto_end_tail
+
+find_theorems "map fst"
+lemma
+  assumes compiler_correct_nt_: True
+  assumes "t_imp = to_imp_tc f_args ctxt bs r stale t"
+  assumes "t_time = time_to_tail reg vs_b vs_arg t"
+  assumes "well_formed_comp f_args ctxt bs stale t"
+  assumes "well_encoded_comp f_args bs vs_arg vs_b s"
+  (* assumes "called_correctness ctxt reg t" *)
+  shows "\<exists>k Cs.
+    (\<exists>t l. tto_end s t_imp k Cs t l)
+    \<and> length Cs = length t_time
+    \<and> (\<forall>((C,s), (g,vs_arg_g)) \<in> set (zip Cs t_time).
+          C = com_from_ctxt ctxt g \<and> vs_arg_g = lookup_args ctxt g s)"
+using assms(2-4) proof (induction t arbitrary: t_imp t_time bs r stale vs_b s)
+  case (hLet t1 t2)
+  then show ?case sorry
+next
+  case (hLetBound x)
+  then show ?case sorry
+next
+  case (hArg x)
+  then show ?case sorry
+next
+  case (hNumber x)
+  then show ?case sorry
+next
+  case (hIf t1 t2 t3)
+  then show ?case sorry
+next
+  case (hCall g ts)
+  let ?xs = "make_n_fresh (length ts) stale ''Call.x.''"
+  let ?cs1 = "mapi (\<lambda>i t. to_imp_tc f_args ctxt bs (?xs ! i) (?xs @ stale) t) ts"
+  let ?cs2 = "mapi (\<lambda>i t. tAssign (args_from_ctxt ctxt g ! i) (A (V (?xs ! i)))) ts"
+  let ?call = "tSeq (tCall (com_from_ctxt ctxt g) (ret_from_ctxt ctxt g)) (tAssign r (A (V (ret_from_ctxt ctxt g))))"
+
+  have "t_imp = t_seqs (?cs1 @ ?cs2) ?call" using hCall by (simp add: Let_def split_beta)
+
+  let ?x = "\<lambda>s. f_from_reg reg g (lookup_args ctxt g s)"
+  have "tto_end s ?call 2 [(com_from_ctxt ctxt g,s)] (s(ret_from_ctxt ctxt g := ?x s, r := ?x s)) False" for s
+    sorry
+
+  then show ?case sorry
+next
+  case (hTAIL x)
+  then show ?case sorry
+qed
+
+
+
+
+    (* \<and> (\<forall>((C,s), (g,vs_arg_g)) \<in> set (zip gs (time_to_tail reg vs_b vs_arg t)). *)
+          (* C = com_from_ctxt ctxt g \<and> vs_arg_g = lookup_args ctxt g s)" *)
+
+
+
 lemma
   assumes compiler_correct_nt_: True
   assumes "t_imp = to_imp_tc f_args ctxt bs r stale t"
@@ -178,7 +354,5 @@ qed
 
 lemma "\<exists>c. \<forall>s. tstruct_k t_imp + something \<le> c * interp_time reg (time_to_tail reg vs_b vs_arg t)" oops
 (* in fact, we can calculate c as the max of the structural-constant-factor and all T_f_const-ants or so *)
-
-
 
 end
